still proving CCAS

examples/CCAS.v
@@ -1,5 +1,6 @@
 Require Import FMapPositive.
 Require Import Relation_Operators Operators_Properties.
+Require Import Coq.Logic.Classical_Prop.
 Require Import Coq.PArith.PArith.
 Require Import Coq.Program.Equality.
 Require Import Lia.
@@ -19,6 +20,26 @@ Require Import RGILogicSet.
 Require Import Specs.
 Require Import SeparationAlgebra.
 
+
+  Ltac split_right :=
+    try (split; [| split_right]).
+
+  Ltac extract n H :=
+    (* let Hneed := fresh "H" in *)
+    lazymatch n with
+      | O => idtac
+      | S ?n' =>
+          destruct H as [_ H];
+          extract n' H
+    end;
+    simpl in H;
+    match H with
+    | exists _, _ => idtac
+    | _ => try destruct H as [H _]
+    end.
+
+  Open Scope nat_scope.
+
 Class HasBeq (t : Type) := {
   beq : t -> t -> bool;
   beq_refl : forall x, beq x x = true;
@@ -26,7 +47,8 @@ Class HasBeq (t : Type) := {
   beq_false : forall x y, beq x y = false -> x <> y;
 }.
 
-Module CASTaskImpl.
+(* TODO: change IsExpired to owner *)
+(* Module CASTaskImpl.
   Import LinCCALBase.
   Import LTSSpec.
   Import Lang.
@@ -66,7 +88,7 @@ Module CASTaskImpl.
   
   Definition tryResolveTask_impl tsk v (_ : tid) : Prog (li_sig E) unit :=
     inl (cas (inl tsk) (inr v)) >= _ => Ret tt.
-End CASTaskImpl.
+End CASTaskImpl. *)
 
 
 Module CCASImpl.
@@ -92,7 +114,7 @@ Module CCASImpl.
   {|
     li_sig := Sig.Plus.omap (ECASTask Val) (EReg bool);
     li_lts := tens_lts VCASTask VReg;
-    li_init := pair (Idle (cts (inr vInit) O nil)) (Idle true);
+    li_init := pair (Idle (cts (inr vInit) O (fun _ => Inactive))) (Idle true);
   |}.
   
   Definition F : layer_interface :=
@@ -112,10 +134,22 @@ Module CCASImpl.
   Definition ALinIdle t : assertion := ALinEx t None.
 
   Definition Flag b : assertion := fun s => state (snd (σ s)) = b.
-  Definition Expired i : assertion := fun s => List.In i (expired (state (fst (σ s)))).
+  Definition IsInactive i : assertion := fun s => owner (state (fst (σ s))) i = Inactive.
+  Definition OwnedBy i t : assertion := fun s => owner (state (fst (σ s))) i = Owned t.
+  Definition IsExpired i : assertion  := fun s => owner (state (fst (σ s))) i = Expired.
   Definition CurrentTask task : assertion := fun s => (current (state (fst (σ s)))) = inl task.
   Definition CurrentVal v : assertion := fun s => (current (state (fst (σ s)))) = inr v.
+  Definition NotPlacedBy i t : assertion :=
+    OwnedBy i t //\\ (∀ o n, !! CurrentTask (CTask t o n i)).
   
+  Lemma OwnedByNotIsExpired : forall i t,
+    ⊨ OwnedBy i t ==>> !! IsExpired i.
+  Proof.
+    intros. intros ? ?.
+    unfold OwnedBy, IsExpired in *.
+    congruence.
+  Qed.
+
   Lemma CurrentTaskCongruence : forall task1 task2 s,
     CurrentTask task1 s -> CurrentTask task2 s -> task1 = task2.
   Proof.
@@ -150,14 +184,14 @@ Module CCASImpl.
   Definition I_cur_task : assertion :=
     ∀ t o n i , CurrentTask (CTask t o n i) ==>>
       (
-        !! Expired i //\\
+        OwnedBy i t //\\
         !! ALinIdle t //\\
         NotDone t o n
       ).
 
   Definition I_not_cur_task : assertion :=
     ∀ t, (∀ o n i, !! CurrentTask (CTask t o n i)) ==>>
-      ((∃ op, ALin t (ls_inv op)) \\// (∃ op r, ALin t (ls_linr op r))).
+      (fun s => exists ls, forall ρ π, Δ s ρ π -> TMap.find t π = ls).
   
   Definition I_flag : assertion :=
     fun s => forall ρ π, Δ s ρ π ->
@@ -167,99 +201,175 @@ Module CCASImpl.
     fun s => forall ρ π, Δ s ρ π ->
       exists s, ρ = Idle s.
 
-  Definition ticket_not_expired : assertion :=
-    fun s => forall t, (ticket (state (fst (σ s)))) <= t ->
-      ~ List.In t (expired (state (fst (σ s)))).
+  Definition ticket_not_owned : assertion :=
+    fun s => forall i, (ticket (state (fst (σ s)))) <= i ->
+      IsInactive i s.
+      (* forall t o n i, ~ CurrentTask (CTask t o n i) s. *)
 
   Definition I : assertion :=
     I_ρ_atomic //\\ I_flag //\\
     I_val //\\ I_cur_task //\\ I_not_cur_task //\\
-    ticket_not_expired.
-
+    ticket_not_owned.
 
   Definition G_trylin : rg_relation :=
-    fun s1 s2 => exists t o n i,
+    fun s1 s2 =>
+      (Δ s1 ⊆ Δ s2)%AbstractConfig /\
+      (exists t o n i, CurrentTask (CTask t o n i) s1) /\
+      forall cts1 cts2,
+        cts1 = state (fst (σ s1)) ->
+        cts2 = state (fst (σ s2)) ->
+        current cts1 = current cts2 /\
+        ticket cts1 = ticket cts2 /\
+        owner cts1 = owner cts2.
+    (* fun s1 s2 => exists t o n i,
       CurrentTask (CTask t o n i) s1 /\
       CurrentTask (CTask t o n i) s2 /\
       (* non-decr when there is task *)
-      (Δ s1 ⊆ Δ s2)%AbstractConfig.
+      (Δ s1 ⊆ Δ s2)%AbstractConfig. *)
 
   Definition G_resolve : rg_relation :=
-    fun s1 s2 => exists t o n i,
+    fun s1 s2 =>
+      (exists v, CurrentVal v s2) /\
+      exists t o n i, CurrentTask (CTask t o n i) s1 /\
+        (exists ρ π,
+          (Δ s2 ≡ [( ρ, π )])%AbstractConfig /\
+          ([( ρ, π )] ⊆ Δ s1)%AbstractConfig /\
+          TMap.find t π = Some (ls_linr (cas o n) o)) /\
+      forall cts1 cts2,
+        cts1 = state (fst (σ s1)) ->
+        cts2 = state (fst (σ s2)) ->
+        ticket cts1 = ticket cts2 /\
+        owner cts1 i = Owned t /\
+        forall i', owner cts2 i' = owner_upd (owner cts1) i Expired i'.
+    (* fun s1 s2 => exists t o n i,
       CurrentTask (CTask t o n i) s1 /\
       (exists v, CurrentVal v s2) /\
-      Expired i s2 /\
+      IsExpired i s2 /\
       (* resolve to single poss with linr *)
       exists ρ π,
         (Δ s2 ≡ [( ρ, π )])%AbstractConfig /\
         ([( ρ, π )] ⊆ Δ s1)%AbstractConfig /\
-        TMap.find t π = Some (ls_linr (cas o n) o).
+        TMap.find t π = Some (ls_linr (cas o n) o). *)
 
-  Definition G_id : rg_relation :=
+  (* Definition G_id : rg_relation :=
     fun s1 s2 =>
       state (fst (σ s1)) = state (fst (σ s2)) /\
       state (snd (σ s1)) = state (snd (σ s2)) /\
-      Δ s1 ≡ Δ s2.
+      Δ s1 ≡ Δ s2. *)
 
-  Definition G_task t : rg_relation :=
-    fun s1 s2 => exists o n i,
+  Definition G_alloc t : rg_relation :=
+    fun s1 s2 =>
+      Δ s1 ≡ Δ s2 /\
+      forall cts1 cts2,
+        cts1 = state (fst (σ s1)) ->
+        cts2 = state (fst (σ s2)) ->
+        current cts1 = current cts2 /\
+        S (ticket cts1) = ticket cts2 /\
+        owner cts1 (ticket cts1) = Inactive /\
+        forall i, owner cts2 i = owner_upd (owner cts1) (ticket cts1) (Owned t) i.
+
+  Definition G_place_task t : rg_relation :=
+    fun s1 s2 =>
+      (exists o n i, CurrentVal o s1 /\
+        CurrentTask (CTask t o n i) s2) /\
+      Δ s1 ≡ Δ s2 /\
+      forall cts1 cts2,
+        cts1 = state (fst (σ s1)) ->
+        cts2 = state (fst (σ s2)) ->
+        ticket cts1 = ticket cts2 /\
+        owner cts1 = owner cts2.
+    (* fun s1 s2 => exists o n i,
       CurrentVal o s1 /\
       CurrentTask (CTask t o n i) s2 /\
-      Δ s1 ≡ Δ s2.
+      Δ s1 ≡ Δ s2 /\
+      OwnedBy i t s1. *)
 
   Definition G t : rg_relation :=
-    G_id ∪ G_task t ∪ G_trylin ∪ G_resolve.
+    G_alloc t ∪ G_place_task t ∪ G_trylin ∪ G_resolve.
 
   (* only the owner can place the task *)
   Definition R_task t : rg_relation :=
     fun s1 s2 => forall o n i,
       ~ CurrentTask (CTask t o n i) s1 -> ~ CurrentTask (CTask t o n i) s2.
 
-  (* Definition R_id t : rg_relation :=
-    fun s1 s2 => 
-      state (fst (σ s1)) = state (fst (σ s2)) /\
-      state (snd (σ s1)) = state (snd (σ s2)) /\
-      forall ls, ALinEx t ls s1 <-> ALinEx t ls s2. *)
+  Definition R_IsExpired : rg_relation :=
+    fun s1 s2 => forall i, IsExpired i s1 -> IsExpired i s2.
 
+  Definition R_notplaced t : rg_relation :=
+    fun s1 s2 => forall i, NotPlacedBy i t s1 -> NotPlacedBy i t s2.
+
+  (* need this to ensure domexact *)
   Definition R_id t : rg_relation :=
-    fun s1 s2 => forall ls, ALinEx t ls s1 <-> ALinEx t ls s2.
+    fun s1 s2 => 
+      forall ls, ALinEx t ls s1 <-> ALinEx t ls s2.
 
   Definition R t : rg_relation :=
-    R_task t ∩
-    (R_id t ∪ G_trylin ∪ G_resolve).
+    R_IsExpired ∩ R_notplaced t ∩
+    ((R_task t ∩ R_id t) ∪ G_trylin ∪ G_resolve).
 
   Lemma RG_compatible : forall t1 t2, t1 <> t2 -> (G t1 ⊆ R t2).
   Proof.
     intros. intros s1 s2 ?.
     destruct H1 as [[[? | ?] | ?] | ?].
-    - split.
-      + destruct H1 as [? [? ?]].
-        unfold R_task, CurrentTask.
-        rewrite H1; auto.
-      + do 2 left.
-        destruct H1 as [? [? ?]].
-        unfold R_id, ALinEx, ALinIdle; intros.
-        split; intros [ρ [π [? ?]]];
-        apply H3 in H4; eauto.
-    - split.
-      + destruct H1 as [? [? [? [? [? ?]]]]].
-        unfold R_task, not. intros.
-        pose proof CurrentTaskCongruence _ _ _ H2 H5.
-        inversion H6. congruence.
-      + do 2 left.
-        destruct H1 as (o & n & i & [? [? ?]]).
-        unfold R_id, ALinEx, ALinIdle; intros.
-        split; intros [ρ [π [? ?]]];
-        apply H3 in H4; eauto.
-    - split; [| left; right; auto].
-      destruct H1 as [? [? [? [? [? [? ?]]]]]].
-      unfold R_task. unfold not at 2. intros.
-      pose proof CurrentTaskCongruence _ _ _ H2 H5.
-      inversion H6; subst. auto.
+    - destruct H1 as [? ?].
+      specialize (H2 _ _ eq_refl eq_refl) as [? [? [? ?]]].
+      split;[split|].
+      + unfold R_IsExpired. unfold IsExpired; intros.
+        rewrite H5. unfold owner_upd. 
+        destruct (Nat.eqb_spec (ticket (state (fst (σ s1)))) i); auto.
+        subst. congruence.
+      + unfold R_notplaced, NotPlacedBy, OwnedBy, CurrentTask, Forall, Neg.
+        intros ? [? ?]. rewrite H2 in *.
+        split; auto.
+        rewrite H5. unfold owner_upd.
+        destruct (Nat.eqb_spec (ticket (state (fst (σ s1)))) i); auto.
+        subst. congruence.
+      + do 2 left. split.
+        * unfold R_task, CurrentTask, Forall.
+          rewrite H2. auto.
+        * unfold R_id, ALinEx.
+          split; intros [? [? [HΔ ?]]];
+          apply H1 in HΔ; do 2 eexists; eauto.
+    - destruct H1 as [[? [? [? [? ?]]]] [? ?]].
+      specialize (H4 _ _ eq_refl eq_refl) as [? ?].
+      split;[split|].
+      + unfold R_IsExpired, IsExpired; intros.
+        rewrite <- H5. auto.
+      + unfold R_notplaced, NotPlacedBy, OwnedBy. intros ? [? ?].
+        rewrite H5 in H6. split; auto.
+        intros ? ? ?.
+        eapply CurrentTaskCongruence in H2; eauto.
+        congruence.
+      + do 2 left. split.
+        * unfold R_task.
+          intros ? ? ? _ ?.
+          eapply CurrentTaskCongruence in H2; eauto. congruence.
+        * unfold R_id, ALinEx.
+          split; intros [? [? [HΔ ?]]];
+          apply H3 in HΔ; do 2 eexists; eauto.
+    - split; [|left; right; auto].
+      destruct H1 as [? [[? [? [? [? ?]]]] ?]].
+      specialize (H3 _ _ eq_refl eq_refl) as [? [? ?]].
+      split.
+      + unfold R_IsExpired, IsExpired.
+        rewrite H5. auto.
+      + unfold R_notplaced, NotPlacedBy, OwnedBy, CurrentTask, Forall, Neg.
+        intros ? [? ?]. rewrite H3 in *. rewrite H5 in *.
+        split; auto.
     - split; [| right; auto].
-      destruct H1 as [? [? [? [? [? [[? ?] ?]]]]]].
-      unfold R_task. unfold not at 2. intros.
-      eapply TaskValConflict; eauto.
+      destruct H1 as [[? ?] [? [? [? [? [? [? ?]]]]]]].
+      specialize (H4 _ _ eq_refl eq_refl) as [? [? ?]].
+      split.
+      + unfold R_IsExpired, IsExpired.
+        intros. rewrite H6.
+        unfold owner_upd. destruct (x3 =? i); auto.
+      + unfold R_notplaced, NotPlacedBy, OwnedBy, CurrentTask, Forall, Neg.
+        intros ? [? ?].
+        split.
+        * rewrite H6.
+          unfold owner_upd. destruct (Nat.eqb_spec x3 i); auto; subst.
+          rewrite H2 in H8. congruence.
+        * rewrite H1. congruence.
   Qed.
 
   Lemma R_domexact : forall t0 s1 s2, R t0 s1 s2 -> I s2 ->
@@ -304,10 +414,10 @@ Module CCASImpl.
   (*
   
   I :=
-      (* current ticket not expired *)
-      ~ In ticket expired //\\
-      (* current task not expired *)
-      (* so that we can easily deduce that the complete method always fail if the task is expired *)
+      (* current ticket not IsExpired *)
+      ~ In ticket IsExpired //\\
+      (* current task not IsExpired *)
+      (* so that we can easily deduce that the complete method always fail if the task is IsExpired *)
       forall i, In i expire -> current <> CTask _ _ _ i
 
       //\\
@@ -320,35 +430,10 @@ Module CCASImpl.
 
   (* 
     G_trylin  : current' = CTask t _ _ _ /\ forall π ∈ Δ, π ∈ Δ'
-    G_resolve : current = CTask t o _ i /\ expired'(i)
+    G_resolve : current = CTask t o _ i /\ IsExpired'(i)
   *)
 
-  (* cid_not_idle := (cid = t //\\ ~ ALinIdle t) \\// cid <> t *)
 
-  Definition complete t o n i : Prog (li_sig E) unit :=
-    (*
-      cid_not_idle //\\
-      task_placed t o n i
-    *)
-    inr Reg'Spec.get >= b =>
-    (*
-      cid_not_idle //\\
-      ((expired(i) //\\ (ALinIdle t \\// ALin t linr o)) \\//
-        (current = CTask t o n i //\\ (exists π ∈ Δ, π ⊨ ALin t linr o)))
-    *)
-    inl (tryResolveTask (CTask t o n i)
-                        (match b with
-                          | true => n
-                          | false => o end)) >= _ =>
-    (* (cid = t //\\ ALin t linr o) \\// cid <> t *)
-    Ret tt.
-  
-
-  (* task_placed t o n i :=
-        cid_not_idle //\\
-        ((expired(i) //\\ (ALinIdle t \\// ALin t linr o)) \\//
-        (current = CTask t o n i //\\ (exists π ∈ Δ, π ⊨ ALin t inv)))
-  *)
 
   Lemma Istable {t} : Stable (R t) I I.
   Proof. unfold Stable. apply ConjRightImpl, ImplRefl. Qed.
@@ -362,26 +447,43 @@ Module CCASImpl.
   Qed.
 
   Lemma ALinExCongruence : forall t ls1 ls2,
-    ⊨ ALin t ls1 ==>> ALinEx t (Some ls2) ==>> ⌜ls1 = ls2⌝.
+    ⊨ ALin t ls1 ==>> ALinEx t ls2 ==>> ⌜Some ls1 = ls2⌝.
   Proof.
     intros. intros ? [? [? [? ?]]].
     apply H0 in H1. congruence.
   Qed.
 
-  Lemma stable_not_cur_task : forall t,
-    Stable (R t) I (∀ o n i, !! CurrentTask (CTask t o n i)).
+
+  Lemma stable_not_cur_task : forall t o n i,
+    Stable (R t) I (!! CurrentTask (CTask t o n i)).
   Proof.
     unfold Stable, R.
     intros. intros [[s0 [? [? ?]]] ?].
     destruct H2 as [[? | ?] | ?].
-    - intros ? ? ?. apply H1, H0.
+    - apply H1, H0.
     - destruct H2 as [? [? [? [? [? [? ?]]]]]].
-      intros o0 n0 i ?.
+      intros ?.
       pose proof CurrentTaskCongruence _ _ _ H4 H6.
       inversion H7; subst. congruence.
     - destruct H2 as (? & ? & ? & ? & [? [[? ?] [? ?]]]).
-      intros ? ? ? ?.
+      intros ?.
       eapply TaskValConflict in H4; eauto.
+  Qed.
+
+  Lemma stable_not_cur_task_oni : forall t,
+    Stable (R t) I (∀ o n i, !! CurrentTask (CTask t o n i)).
+  Proof.
+    intros.
+    do 3 (apply StableForall; intros).
+    apply stable_not_cur_task.
+  Qed.
+
+  Lemma stable_not_cur_task_on : forall t i,
+    Stable (R t) I (∀ o n, !! CurrentTask (CTask t o n i)).
+  Proof.
+    intros.
+    do 2 (apply StableForall; intros).
+    apply stable_not_cur_task.
   Qed.
 
   Lemma stable_ccas_l0: forall t o n,
@@ -391,38 +493,205 @@ Module CCASImpl.
     unfold Stable, R.
     intros. intros ?.
     assert ((∀ (o0 n0 : Val) (i : nat), !! CurrentTask (CTask t0 o0 n0 i)) s);
-    [eapply StableWeaken; eauto;[apply stable_not_cur_task| |]; solve_conj_impl |].
+    [eapply StableWeaken; eauto;[apply stable_not_cur_task_oni| |]; solve_conj_impl |].
     split; auto.
     destruct H0 as [[s0 [[? ?] [? ?]]] ?].
     destruct H4 as [[? | ?] | ?].
     - unfold R_id in H4.
-      apply H5 in H1 as [[? ?] | [? [? ?]]].
-      + pose proof H1.
-        apply ALinALinEx in H1.
-        apply H4 in H1.
-        eapply ALinExCongruence in H1; eauto.
-        inversion H1; subst; auto.
-      + apply ALinALinEx in H1.
-        apply H4 in H1.
-        eapply ALinExCongruence in H1; eauto.
-        congruence.
+      intros ? ? ?.
+      assert (TMap.find t0 π = Some (ls_inv (cas o n)) \/ TMap.find t0 π <> Some (ls_inv (cas o n))) as [? | ?] by apply classic; auto.
+      assert (ALinEx t0 (TMap.find t0 π) s); [do 2 eexists; eauto|].
+      apply H4 in H8.
+      eapply ALinExCongruence in H8; eauto.
     - destruct H4 as [? [? [? [? [? [? ?]]]]]].
-      apply H5 in H1 as [[? ?] | [? [? ?]]];
-      [assert (x3 = cas o n); subst; auto|];
-      pose proof ac_nonempty (Δ s0) as [? [? ?]];
-      pose proof H8;
-      apply H0 in H8;
-      apply H7, H1 in H9;
-      change (li_sig F) with (ECCAS Val) in H9;
-      congruence.
+      apply H5 in H1 as [? ?].
+      pose proof ac_nonempty (Δ s0) as [? [? ?]].
+      pose proof H8.
+      apply H7 in H8.
+      apply H0 in H9.
+      intros ? ? ?.
+      apply H1 in H10, H8.
+      change (li_sig F) with (ECCAS Val) in H8.
+      rewrite H8 in H9; subst.
+      rewrite H9 in H10; auto.
     - destruct H4 as (? & ? & ? & ? & [? [[? ?] [? ?]]]).
       destruct H8 as [ρ [π [? [? ?]]]].
       intros ? ? ?.
       apply H8, H9, H0 in H11; auto.
   Qed.
 
+  Lemma stable_ccas_l1: forall t i,
+    Stable (R t) I
+      (!! IsExpired i //\\ ∀ o n, !! CurrentTask (CTask t o n i)).
+  Proof.
+    unfold Stable, R.
+    intros. intros ?.
+    assert ((∀ (o0 n0 : Val) (i : nat), !! CurrentTask (CTask t0 o0 n0 i)) s);
+    [eapply StableWeaken; eauto;[apply stable_not_cur_task_oni| |]; solve_conj_impl |].
+    split; auto.
+    destruct H0 as [[s0 [[? ?] [? ?]]] ?].
+    destruct H4 as [[? | ?] | ?].
+    - unfold R_id in H4.
+      intros ? ? ?.
+      assert (TMap.find t0 π = Some (ls_inv (cas o n)) \/ TMap.find t0 π <> Some (ls_inv (cas o n))) as [? | ?] by apply classic; auto.
+      assert (ALinEx t0 (TMap.find t0 π) s); [do 2 eexists; eauto|].
+      apply H4 in H8.
+      eapply ALinExCongruence in H8; eauto.
+    - destruct H4 as [? [? [? [? [? [? ?]]]]]].
+      apply H5 in H1 as [? ?].
+      pose proof ac_nonempty (Δ s0) as [? [? ?]].
+      pose proof H8.
+      apply H7 in H8.
+      apply H0 in H9.
+      intros ? ? ?.
+      apply H1 in H10, H8.
+      change (li_sig F) with (ECCAS Val) in H8.
+      rewrite H8 in H9; subst.
+      rewrite H9 in H10; auto.
+    - destruct H4 as (? & ? & ? & ? & [? [[? ?] [? ?]]]).
+      destruct H8 as [ρ [π [? [? ?]]]].
+      intros ? ? ?.
+      apply H8, H9, H0 in H11; auto.
+  Qed.
 
+    Open Scope nat.
 
+  Lemma Ginv_I : forall t f, ⊨ Ginv t f ⊚ I ==>> I.
+  Proof.
+    intros. intros [s' [HI [Hσ [? HΔ]]]].
+    unfold I in *.
+    split_right.
+    - extract 0 HI. unfold I_ρ_atomic in *.
+      intros.
+      apply HΔ in H1. inversion H1; subst.
+      eapply HI; eauto.
+    - extract 1 HI. unfold I_flag in *.
+      intros.
+      apply HΔ in H1. inversion H1; subst.
+      rewrite Hσ in *.
+      eapply HI; eauto.
+    - extract 2 HI. unfold I_val, CurrentVal in *.
+      intros.
+      apply HΔ in H2. inversion H2; subst.
+      rewrite Hσ in *.
+      eapply HI; eauto.
+    - extract 3 HI. unfold I_cur_task, CurrentTask in *.
+      intros ? ? ? ? ?.
+      rewrite <- Hσ in *. apply HI in H1.
+      split_right; unfold IsExpired, ALinIdle, NotDone in *.
+      + extract 0 H1. unfold Neg in *. rewrite <- Hσ in *. auto.
+      + extract 1 H1. intros [? [? [? ?]]]. apply H1.
+        apply HΔ in H2. inversion H2; subst.
+        do 2 eexists; split; eauto.
+        rewrite TMap.gso in H3; auto.
+        intros ?; subst.
+        rewrite TMap.gss in H3. congruence.
+      + destruct H1 as [_ [_ [? [? [? [? ?]]]]]].
+        exists x, (TMap.add t0 (ls_inv f) x0); split_right; auto.
+        * apply HΔ. constructor; auto.
+        * rewrite TMap.gso; auto.
+          intros ?; subst.
+          apply H0 in H1; congruence.
+    - extract 4 HI. unfold I_not_cur_task, CurrentTask in *.
+      intros ? ?. unfold Forall, Neg in H1. rewrite <- Hσ in H1.
+      apply HI in H1 as [? ?].
+      destruct (Pos.eq_dec v t0); subst.
+      + exists (Some (ls_inv f)); intros.
+        apply HΔ in H2; inversion H2; subst.
+        rewrite TMap.gss; auto.
+      + exists x; intros.
+        apply HΔ in H2; inversion H2; subst.
+        rewrite TMap.gso; eauto.
+    - extract 5 HI. unfold ticket_not_owned in *.
+      rewrite Hσ in *. apply HI in H1 as [? ?]. eauto.
+    - extract 5 HI. unfold ticket_not_owned in *.
+      rewrite Hσ in *. apply HI in H1 as [? ?].
+      unfold CurrentTask in *. rewrite Hσ in *.
+      eauto.
+  Qed.
+
+  Lemma Gret_I : forall t f ret,
+    ⊨ Gret t f ret ⊚ (I //\\ ALin t (ls_linr f ret)) ==>> I.
+  Proof.
+    intros. intros [s' [[HI HALin] [Hσ [? HΔ]]]].
+    unfold I in *.
+    split_right.
+    - extract 0 HI. unfold I_ρ_atomic in *.
+      intros.
+      apply HΔ in H1. inversion H1; subst.
+      eapply HI; eauto.
+    - extract 1 HI. unfold I_flag in *.
+      intros.
+      apply HΔ in H1. inversion H1; subst.
+      rewrite Hσ in *.
+      eapply HI; eauto.
+    - extract 2 HI. unfold I_val, CurrentVal in *.
+      intros.
+      apply HΔ in H2. inversion H2; subst.
+      rewrite Hσ in *.
+      eapply HI; eauto.
+    - extract 3 HI. unfold I_cur_task, CurrentTask in *.
+      intros ? ? ? ? ?.
+      rewrite <- Hσ in *. apply HI in H1.
+      split_right; unfold IsExpired, ALinIdle, NotDone in *.
+      + extract 0 H1. unfold Neg in *. rewrite <- Hσ in *. auto.
+      + pose proof H1. extract 1 H1. destruct H2 as [_ [_ ?]].
+        intros [? [? [? ?]]]. apply H1.
+        apply HΔ in H3. inversion H3; subst.
+        do 2 eexists; split; eauto.
+        rewrite TMap.gro in H4; auto.
+        intros ?; subst.
+        destruct H2 as [? [? [? [? ?]]]].
+        apply H0 in H2. congruence.
+      + destruct H1 as [_ [_ [? [? [? [? ?]]]]]].
+        exists x, (TMap.remove t0 x0); split_right; auto.
+        * apply HΔ. constructor; auto.
+        * rewrite TMap.gro; auto.
+          intros ?; subst.
+          apply H0 in H1; congruence.
+    - extract 4 HI. unfold I_not_cur_task, CurrentTask in *.
+      intros ? ?. unfold Forall, Neg in H1. rewrite <- Hσ in H1.
+      apply HI in H1 as [? ?].
+      destruct (Pos.eq_dec v t0); subst.
+      + exists None; intros.
+        apply HΔ in H2; inversion H2; subst.
+        rewrite TMap.grs; auto.
+      + exists x; intros.
+        apply HΔ in H2; inversion H2; subst.
+        rewrite TMap.gro; eauto.
+    - extract 5 HI. unfold ticket_not_owned in *.
+      rewrite Hσ in *. apply HI in H1 as [? ?]. eauto.
+    - extract 5 HI. unfold ticket_not_owned in *.
+      rewrite Hσ in *. apply HI in H1 as [? ?].
+      unfold CurrentTask in *. rewrite Hσ in *.
+      eauto.
+  Qed.
+            
+
+  (* cid_not_idle := (cid = t //\\ ~ ALinIdle t) \\// cid <> t *)
+  (* task_placed t o n i :=
+      cid_not_idle //\\
+      ((IsExpired i //\\ (ALinIdle t \\// ALin t linr o)) \\//
+      (current = CTask t o n i //\\ NotDone t o n i))
+  *)
+
+  Definition complete t o n i : Prog (li_sig E) unit :=
+    (*
+      cid_not_idle //\\
+      task_placed t o n i
+    *)
+    inr Reg'Spec.get >= b =>
+    (*
+      cid_not_idle //\\
+      ((IsExpired i //\\ (ALinIdle t \\// ALin t linr o)) \\//
+        (current = CTask t o n i //\\ ALinEx t linr o))
+    *)
+    inl (tryResolveTask (CTask t o n i)
+                        (match b with
+                          | true => n
+                          | false => o end)) >= _ =>
+    (* (cid = t //\\ ALin t linr o) \\// cid <> t *)
+    Ret tt.
 
   Definition ccas_impl o n (cid : tid) : Prog (li_sig E) Val :=
     (* I:= ... //\\ ALin t None -> current <> CTask t _ _ _ //\\ ... *)
@@ -431,11 +700,8 @@ Module CCASImpl.
     *)
     inl (allocTask o n) >= i =>
     (* ILoop :=
-      ALin t inv //\\ 
-      (* stable because current <> CTask t _ _ i *)
-      ~ expired(i) //\\
-      (* stable because only t can set current to CTask t _ _ _ *)
-      current <> CTask t _ _ i
+      ALin t inv //\\ current <> CTask t _ _ _ //\\
+      OwnedBy i t //\\ current <> CTask _ _ _ i
     *)
     Do {
       inl (tryPlaceTask o n i) >= r =>
@@ -445,7 +711,7 @@ Module CCASImpl.
           r <> o //\\ r = task t' o' n' i' //\\ task_placed t' o' n' i' //\\ t' <> t)
         (* the following cases will break the loop *)
         (* failed *)
-        (r <> o //\\ isVal r //\\ alin t (linr ccas r))
+        (r <> o //\\ isVal r //\\ ALin t (linr ccas r))
         (* my task *)
         (r = o //\\ task_placed t o n i //\\ ~ ALinIdle t)
       *)
@@ -460,14 +726,14 @@ Module CCASImpl.
           Ret r
       (* 
         (* failed *)
-        (r <> o //\\ isVal r //\\ Alin t (linr ccas r))
+        (r <> o //\\ isVal r //\\ ALin t (linr ccas r))
         (* my task *)
         (r = o //\\ task_placed t o n //\\ ~ ALinIdle t)
       *)
       | _ => Ret r
       end
     } Loop >= r =>
-    (if beq r o then
+    ((if beq r o then
       (*
         r = o //\\ task_placed t o n //\\ ~ ALinIdle t
       *)
@@ -477,10 +743,10 @@ Module CCASImpl.
       *)
     else
       (*
-        Alin t (linr ccas r)
+        ALin t (linr ccas r)
       *)
       Ret tt) ;;
-    Ret r.
+    Ret r).
 
   Definition setFlag_impl b (_ : tid) : Prog (li_sig E) unit :=
     inr (set b) >= _ => Ret tt.
@@ -489,6 +755,17 @@ Module CCASImpl.
   Create HintDb stableDB.
   Hint Resolve stable_ccas_l0 Istable : stableDB.
 
+  (* Ltac extract n H :=
+    (* let Hneed := fresh "H" in *)
+    lazymatch n with
+      | O => idtac
+      | S ?n' =>
+          destruct H as [_ H];
+          extract n' H
+    end;
+    try destruct H as [H _]. *)
+
+    
   Program Definition MCCAS : layer_implementation E F := {|
     li_impl m :=
       match m with
@@ -554,7 +831,46 @@ Module CCASImpl.
         constructor;
         try solve_conj_impl;
         try solve_conj_stable' stableDB.
+        (* invocation *)
+        {
+          intros ? ?.
+          split; [apply Ginv_I in H0; auto|].
+          destruct H0 as [s' [HI [Hσ [? HΔ]]]].
+          split.
+          - intros ? ? ?.
+            apply HΔ in H1. inversion H1; subst.
+            rewrite TMap.gss. auto.
+          - intros ? ? ? ?.
+            unfold I in HI. extract 3 HI.
+            unfold I_cur_task, CurrentTask in *.
+            rewrite <- Hσ in *. apply HI in H1 as [_ [_ ?]].
+            destruct H1 as [? [? [? [? ?]]]].
+            apply H0 in H1. congruence.
+        }
+        (* response *)
+        {
+          intros. intros [? [[? ?] ?]].
+          eapply Gret_I; eexists; do 2 (split; eauto).
+        }
+        {
+          intros. apply H0 in H1. auto.
+        }
 
+        unfold ccas_impl. simpl.
+
+        (* allocTask *)
+        eapply provable_vis_safe with
+          (P' := I //\\
+                ALin t (ls_inv (cas o n)) //\\
+                (∀ (o0 n0 : Val) (i : nat), !! CurrentTask (CTask t o0 n0 i)))
+          (Q' := fun i => I //\\
+                ALin t (ls_inv (cas o n)) //\\
+                !! IsExpired (i) //\\
+                (∀ (o0 n0 : Val), !! CurrentTask (CTask t o0 n0 i)));
+          try solve_no_error;
+          try solve_conj_impl;
+          try solve_conj_stable stableDB.
+          [solve_no_error | | |].
       }
     }
 
@@ -568,9 +884,9 @@ Module CCASImpl.
     Do {
       (*
         I //\\ alin t (inv ccas) 
-        (* my ticket is not expired *)
+        (* my ticket is not IsExpired *)
         (* other wise it breaks the invariant *)
-        //\\ ~ In i expired
+        //\\ ~ In i IsExpired
       *)
       inl (tryPlaceTask o n i) >= r =>
       (* I //\\ 
